Proof that a 3-d random walk is transient.
![[Screenshot 2023-11-25 at 11.12.37â€¯PM.png#invert|400]]
keywords: probability, gambler random walk drunk bird drunk man 2d 3d #math/prob #math/prob #math/prob/markov 
# Math exch qn
https://math.stackexchange.com/questions/4814423/summation-coming-about-in-the-process-of-solving-a-3d-random-walk-sum-limits/4814461#4814461
and
https://math.stackexchange.com/questions/4814507/how-to-get-asymptotic-approximations-for-complex-summations-like-s-n-sum-lim

I'm looking for a closed form for the summation:

$$S_n = \sum\limits_{i=0}^n {n \choose i}^2 {2(n-i)\choose (n-i)}$$

_________________
Why do I care about this summation? It comes about as I'm trying to get a closed form for the 3-d random walk (a drunk bird). This is extending the approach used in example 4.18 of the book Introduction to Probability models by Sheldon Ross (10th edition) for determining if 1-d and 2-d random walks are transient or recurrent.

The probability that a 3-d random walk where the probabilities of moving along the positive and negative x, y and z-axes are equal returning to the origin after taking $2n$ steps is:

$$P^{2n}_{00} = \sum\limits_{i+j\leq n} \frac{(2n)!}{(i!)^2(j!)^2((n-i-j)!)^2}\frac{1}{6^{2n}}$$

The expected number of times the walk comes back to the origin when its run for an infinite number of steps becomes:

$$E_{000} = \sum\limits_{n=1}^\infty \sum\limits_{i=0}^n \sum\limits_{j=0}^{(n-i)} \frac{(2n)!}{(i!)^2(j!)^2((n-i-j)!)^2}\frac{1}{6^{2n}}$$

$$\begin{align}E_{000} = \sum\limits_{n=1}^\infty \frac{(2n)!}{6^{2n}}\sum\limits_{i=0}^n \frac{1}{(i!)^2}\sum\limits_{j=0}^{(n-i)} \frac{1}{(j!)^2((n-i-j)!)^2}\\
= \sum\limits_{n=1}^\infty \frac{(2n)!}{6^{2n}}\sum\limits_{i=0}^n \frac{1}{(i!)^2((n-i)!)^2}\sum\limits_{j=0}^{(n-i)} \frac{((n-i)!)^2}{(j!)^2((n-i-j)!)^2}\\
= \sum\limits_{n=1}^\infty \frac{(2n)!}{6^{2n}}\sum\limits_{i=0}^n \frac{1}{(i!)^2((n-i)!)^2}\sum\limits_{j=0}^{(n-i)} {n-i \choose j}^2\\
= \sum\limits_{n=1}^\infty \frac{(2n)!}{(n!)^2}\frac{1}{6^{2n}}\sum\limits_{i=0}^n \frac{(n!)^2}{(i!)^2((n-i)!)^2}{2(n-i) \choose (n-i)}\\
= \sum\limits_{n=1}^\infty \frac{(2n)!}{(n!)^2}\frac{1}{6^{2n}}\sum\limits_{i=0}^n {n \choose i}^2{2(n-i) \choose (n-i)}\\
= \sum\limits_{n=1}^\infty \frac{(2n)!}{(n!)^2}\frac{1}{6^{2n}}\sum\limits_{i=0}^n {n \choose i}^2{2(n-i) \choose (n-i)}\\
= \sum\limits_{n=1}^\infty \frac{(2n)!}{(n!)^2}\frac{1}{6^{2n}}S_n
\end{align}$$

$$E_{0,0,0}= \sum\limits_{n=1}^\infty \frac{(2n)!}{(n!)^2}\frac{1}{6^{2n}}S_n$$

$$S_n = \sum\limits_{i=0}^n {n \choose i}^2{2(n-i) \choose (n-i)}$$

Where $S_n$ is our summation of interest.

$$F_{0,0,0} = $$
$$\sum\limits_{i=0}^n {n \choose i}^2 = \sum\limits_{i=0}^n {n \choose i}{n \choose {n-i}} = {2n \choose n}$$

$$\frac{(2n)!}{(n!)^2} \sim \frac{4^n}{\sqrt{\pi n}}$$
$$E_{0,0,0} \sim \sum\limits_{n=1}^\infty\frac{36^n}{36^n} \frac{3^{\frac 3 2}}{4(\pi n)^{\frac 3 2}} = c. \zeta\left(\frac{3}{2}\right)$$

